case_studies/minivec/output/minivec/proofs/proof_RawVec_T_grow.v
@@ -22,13 +22,6 @@ Proof.
   Unshelve. all: sidecond_solver.
   Unshelve. all: sidecond_hammer.
   { unfold size_of_array_in_bytes in *. simplify_layout_assum. nia. }
-  {
-    revert select (ly_size (mk_array_layout _ _) ≤ _).
-    move: Hnot_sz.
-    match goal with H : 2 * MaxInt ISize < MaxInt USize |- _ => move: H end.
-    rewrite ly_size_mk_array_layout.
-    clear. solve_goal with nia.
-  }
 
   Unshelve. all: print_remaining_sidecond.
 Qed.
