theories/rust_typing/automation/proof_state.v
@@ -212,21 +212,6 @@ repeat match goal with
 | H : use_union_layout_alg _ = _ |- _ => clear H
 end.
 
-Ltac prepare_sideconditions :=
-  li_unfold_lets_in_context;
-  unfold_instantiated_evars;
-  repeat match goal with | H : BLOCK_PRECOND _ _ |- _ => clear H end;
-  (* get rid of Q *)
-  repeat match goal with | H := CODE_MARKER _ |- _ => clear H end;
-  repeat match goal with | H := RETURN_MARKER _ |- _ => clear H end;
-  unfold_no_enrich;
-  clear_layout;
-  clear_unused_vars.
-
-Ltac solve_goal_prepare_hook ::=
-  prepare_sideconditions;
-  repeat match goal with | H : CASE_DISTINCTION_INFO _ |- _ =>  clear H end.
-
 (** * Tactics for showing failures to the user *)
 
 (*Ltac print_current_location :=*)
